Further work on definitions and lemmas required for the main_unification_theorem. Changed some previous definitions and lemmas. Main changes: Seperation of fomal and concrete unification steps, as well as a formal definition of a solved Equality Problem. Still work in progress

InferenceInLean/D_Unification.lean
@@ -3,7 +3,7 @@ import InferenceInLean.B_Semantics
 import InferenceInLean.C_Models
 
 set_option autoImplicit false
---set_option diagnostics true
+set_option diagnostics false
 
 open Syntax
 open Semantics
@@ -13,19 +13,21 @@ open Models
 
 namespace Unification
 
-@[simp]
-def Equality (sig : Signature) (X : Variables) :=
-  Term sig X × Term sig X
 
 @[simp]
-def EqualityProblem (sig : Signature) (X : Variables) :=
+abbrev Equality (sig : Signature) (X : Variables) :=
+Term sig X × Term sig X
+
+@[simp]
+abbrev EqualityProblem (sig : Signature) (X : Variables) :=
   List (Equality sig X)
 
 instance {sig : Signature} {X : Variables} : Membership (Equality sig X) (EqualityProblem sig X) :=
   List.instMembership
 
 @[simp]
-def EqualityProblem.freeVars {sig : Signature} {X : Variables} : EqualityProblem sig X -> Set X
+def EqualityProblem.freeVars {sig : Signature} {X : Variables} [DecidableEq X] :
+    EqualityProblem sig X -> Set X
   | [] => ∅
   | (lhs, rhs) :: eqs => Term.freeVars sig X lhs ∪ Term.freeVars sig X rhs ∪ freeVars eqs
 
@@ -55,98 +57,332 @@ lemma mgu_imp_unifier {sig : Signature} {X : Variables} [DecidableEq X] (E : Equ
 def Unifiable {sig : Signature} {X : Variables} [DecidableEq X]
   (E : EqualityProblem sig X) : Prop := ∃ σ : Substitution sig X, Unifier E σ
 
-theorem unifiable_iff_mgu_idempot {sig : Signature} {X : Variables} [inst : DecidableEq X]
-    (E : EqualityProblem sig X) : Unifiable E ↔ ∃ σ : Substitution sig X,
-      MostGeneralUnifier E σ ∧ Idempotent σ ∧ σ.domain ∪ σ.codomain ⊆ E.freeVars := by
-  apply Iff.intro
-  · sorry
-    /- This direction would need the standard unification algorithm.
-    I have played around with implementing it but it brings quite some chanllenge with it and feels
-    like it's outside the scope of this project.
-      -/
-  · intro h
-    obtain ⟨σ, ⟨⟨⟩⟩⟩ := h
-    use σ
-alias main_unification_theorem := unifiable_iff_mgu_idempot
 
 
-/- Rule-Based Naive Standard Unification Algorithm -/
-
-def var_includes {sig : Signature} {X : Variables} [DecidableEq X] (s : Term sig X) (var : List X) : Bool :=
-match s with
-  | Term.var x => (x ∈ var)
-  | _ => false
-
-def term_includes {sig : Signature} {X : Variables} [DecidableEq X] (s : Term sig X) (x : X) : Bool :=
-match s with
-  | Term.var y => (x == y)
-  | Term.func _ [] => false
-  | Term.func f (a :: args) =>
-      if (term_includes a x) then true
-      else (term_includes (Term.func f args) x)
-
-def E_includes {sig : Signature} {X : Variables} [DecidableEq X] (E : EqualityProblem sig X) (x : X) : Bool :=
-match E with
-  | [] => false
-  | (s, t) :: args =>
-      if ((term_includes s x) || (term_includes t x)) then true
-      else (E_includes args x)
 
 
-def decomposition {sig : Signature} {X : Variables} (E : EqualityProblem sig X) (args bargs: List (Term sig X)) : EqualityProblem sig X :=
 
-  let rec decomposition_rec (E : EqualityProblem sig X) (args bargs: List (Term sig X)) : EqualityProblem sig X :=
-    match args, bargs with
-      | (a :: aa), (b :: bb) =>
-        let e : Equality sig X := (a, b)
-        decomposition_rec (e :: E) aa bb
-      | _, _ => E
 
-decomposition_rec E args bargs
+----------------------------------------------------------------------------------------------------
+--The project is still work in progress and therefore definitions and lemmas may include mistakes --
+----------------------------------------------------------------------------------------------------
 
-/-Termination proof still to be done; tried out different approaches so far but Lean still cannot observe eventual termination.
-  Therefore, the definition is for now partial -/
-def standard_unification_steps {sig : Signature} {X : Variables} [DecidableEq X] [BEq sig.funs]
-(E : EqualityProblem sig X) (var: List X) (σ : Substitution sig X) : Option (EqualityProblem sig X × Substitution sig X) :=
+
+
+
+
+----------------------------
+--Unification algoirthm --
+----------------------------
+
+/-One formal step of the unification algorithm:
+  Based on Christian Sternagel and René Thiemann's Isabelle implementation of (abstract) unification:
+  https://www.isa-afp.org/sessions/first_order_terms/#Abstract_Unification.html &
+  https://www.isa-afp.org/sessions/first_order_terms/#Unification.html. License : LGPL -/
+
+def sub_E {sig : Signature} {X : Variables} [DecidableEq X] (σ : Substitution sig X) [DecidableEq X] : EqualityProblem sig X -> EqualityProblem sig X
+| [] => []
+| (s,t) :: E => ((s.substitute σ, t.substitute σ) :: (sub_E σ E))
+
+inductive Unification_Step  {sig : Signature} {X : Variables} [DecidableEq X] [BEq (sig.funs)]
+: Substitution sig X -> EqualityProblem sig X -> EqualityProblem sig X -> Prop
+where
+| refl (t : Term sig X) (E: EqualityProblem sig X) (σ : Substitution sig X) : (Unification_Step σ ((t,t) :: E) E)
+| decomposition  (f : sig.funs) (args brgs : List (Term sig X)) (E : EqualityProblem sig X) (σ : Substitution sig X)
+  (len: args.length = brgs.length) : (Unification_Step σ ((Term.func f args, Term.func f brgs) :: E) ((List.zip args brgs) ++ E))
+| var_left  (x : X) (t : Term sig X) (E : EqualityProblem sig X) (σ : Substitution sig X) (not_in : (x ∉ Term.freeVarsList sig X t)) :
+  (Unification_Step  (σ.modify x t) ((Term.var x, t) :: E) (sub_E (σ.modify x t) E))
+| var_right (x : X) (t : Term sig X) (E : EqualityProblem sig X) (σ : Substitution sig X) (not_in : (x ∉ Term.freeVarsList sig X t))  :
+  (Unification_Step  (σ.modify x t) ((t,Term.var x) :: E) (sub_E (σ.modify x t) E))
+
+----------------------
+
+--One concret step of the unification algorithm --
+
+def Naive_Standard_Unification {sig : Signature} {X : Variables} [DecidableEq X] [BEq sig.funs]
+ (E : EqualityProblem sig X) (σ : Substitution sig X) : Option (EqualityProblem sig X × Substitution sig X) :=
 
 match E with
+
 | [] => some ([], σ)
 | (s, t) :: E' =>
 
-  let s' := (s.substitute σ)
-  let t' := (t.substitute σ)
+  if eqTerm sig X s t then some (E', σ)
 
-  if (eqTerm sig X s' t') then some (E', σ)
+  else match s, t with
 
-  else let (s'', t'') :=
-    match s', t' with
-      | _, Term.var y => if ¬(var_includes s' var) then (Term.var y, s') else (s', t')
-      | _, _ => (s', t')
-
-    match s'', t'' with
-
-    | Term.func f args, Term.func g bargs =>
-      if (f == g) && (args.length == bargs.length)
-        then let Eq := (decomposition E args bargs)
-        some (Eq,σ)
+    | Term.func f args, Term.func g gargs =>
+      if (f == g) ∧ (args.length == gargs.length)
+      then some ((List.zip args gargs) ++ E', σ)
       else none
 
-    | Term.var x, _ =>
-      if (E_includes E x) && ¬(term_includes t'' x) then
-        let hσ := (σ.modify x t'')
-        let E' := E.map (fun (s,t) => (s.substitute hσ, t.substitute hσ))
-        let e : Equality sig X := (Term.var x, t'')
-        some ((e::E'), σ)
-      else if (term_includes t'' x) && ¬(eqTerm sig X s'' t'') then none
+    | Term.func _ _, Term.var x =>
+      if (x ∉ Term.freeVarsList sig X s)
+      then
+        let hσ := σ.modify x s
+        some ((sub_E hσ E'), hσ)
       else none
 
-    | Term.func _ _, Term.var _ => none
+    | Term.var x, t'  =>
+      if (x ∉ Term.freeVarsList sig X t')
+      then
+        let hσ := σ.modify x t'
+        some (sub_E hσ E', hσ)
+      else none
+
+--Unification algorithm recursion --
+
+partial def Naive_Standard_Unification_Rec {sig : Signature} {X : Variables} [DecidableEq X] [BEq sig.funs]
+ (E : EqualityProblem sig X) (σ : Substitution sig X) : Option (Substitution sig X) :=
+
+ match Naive_Standard_Unification E σ with
+  | none => none
+  | some ([], σ') => some σ'
+  | some (E', σ') => Naive_Standard_Unification_Rec E' σ'
+
+-- Initial substitution to start the algorithm --
+
+def initSubst {sig : Signature} {X : Variables} : Substitution sig X := fun x => Term.var x
+
+def initStart {sig X} [DecidableEq X] [BEq sig.funs] (E : EqualityProblem sig X) : Option (Substitution sig X) :=
+Naive_Standard_Unification_Rec E initSubst
+
+-- Unification_Step formalizes concrete steps of Naive_Standard_Unification --
+
+lemma Unify_Step  {sig : Signature} {X : Variables} [DecidableEq X] [BEq sig.funs] (E E' : EqualityProblem sig X)
+(σ σ' : Substitution sig X) (algo : Naive_Standard_Unification E σ = some (E', σ')) : Unification_Step σ E E' := by
+sorry
 
 
-partial def standard_unification {sig : Signature} {X : Variables} [DecidableEq X] [BEq sig.funs]
-(E : EqualityProblem sig X) (var: List X) (σ : Substitution sig X) : Option (Substitution sig X) :=
+------------------------------------------------------------------------
+--Proposition 3.10.3 & required definitions:
+--If an EqualityProblem is in a SolvedForm then the Solution Sigma_Solved
+--is a Most General Unifier of this EqualityProblem
+------------------------------------------------------------------------
 
-match (standard_unification_steps E var σ) with
-| none => none
-| some ([], σ') => some σ'
-| some (E', σ') => (standard_unification E' var σ')
+def Solved_Form {sig : Signature} {X : Variables} [DecidableEq X] (E : EqualityProblem sig X) : Prop :=
+(∀ s t, (s, t) ∈ E -> ∃ x, s = Term.var x) ∧ --only variables on the left side
+(∀ x t₁ t₂, (Term.var x, t₁) ∈ E -> (Term.var x, t₂) ∈ E -> (t₁ = t₂)) ∧ -- pairwise distinctness
+(∀ x t, (Term.var x, t) ∈ E -> (x ∉ Term.freeVarsList sig X t)) -- no left-sided variables included in the term variables
+
+def Sigma_Solved  {sig : Signature} {X : Variables} [DecidableEq X] (E : EqualityProblem sig X) : Substitution sig X :=
+match E with
+| [] => fun x => Term.var x
+| (Term.var x, t) :: E' =>
+    let σ := Sigma_Solved E'
+    let t' := t.substitute σ
+    σ.modify x t'
+| _ :: E' => Sigma_Solved E'
+
+lemma Solution {sig : Signature} {X : Variables} [DecidableEq X] (E:EqualityProblem sig X) (solved : Solved_Form E) :
+Unifier E (Sigma_Solved E) := by
+sorry
+
+lemma Sigma {sig : Signature} {X : Variables} [DecidableEq X] (E:EqualityProblem sig X) (solved : Solved_Form E)
+(τ : Substitution sig X) (hτ : Unifier E τ) : Sigma_Solved E ≤ τ := by
+sorry
+
+lemma Most_General_Sigma_Solved {sig : Signature} {X:Variables} [DecidableEq X] (E : EqualityProblem sig X) (solved : Solved_Form E) :
+MostGeneralUnifier E (Sigma_Solved E) := by
+constructor
+· exact (Solution E solved)
+· intro τ hτ
+  exact (Sigma E solved τ hτ)
+
+--Proposition 3.10.3 implies : if a MGU exists, then the resulting EquationProblem E' is in a Solved_Form with a Sigma_Solved for E'
+lemma Ex_SolvedForm_Sigma {sig : Signature} {X : Variables} [DecidableEq X] [BEq sig.funs] (E : EqualityProblem sig X) (σ' : Substitution sig X)
+(algo : Naive_Standard_Unification_Rec E initSubst = some σ') : ∃ E', Solved_Form E' ∧ (σ' = Sigma_Solved E') := by
+sorry
+
+-------------------------------------------------------------------------------------------------------
+--Theorem 3.10.4
+-- 1. If UNIF1 σ E E' / Naive_Standard_Unification then (∀ τ is a Unifier of E <-> τ is a Unifier of E')
+-------------------------------------------------------------------------------------------------------
+
+lemma unifier_eq_step {sig : Signature} {X : Variables} [DecidableEq X] [BEq sig.funs] (E E' : EqualityProblem sig X)
+(σ : Substitution sig X) (hUNIF : Unification_Step σ E E') : (∀ τ,  Unifier E τ ↔ Unifier E' τ) := by
+intro τ
+induction hUNIF with
+| refl => simp [Unifier]
+| decomposition f args bargs E σ hlen => sorry
+| var_left x t E σ not_in => sorry
+| var_right x t E σ not_in => sorry
+
+lemma unifier_eq_algorithm {sig : Signature} {X : Variables} [DecidableEq X] [BEq sig.funs] (E E' : EqualityProblem sig X)
+(σ σ' : Substitution sig X) (algo : Naive_Standard_Unification E σ = some (E', σ')) : ∀ τ, Unifier E τ ↔ Unifier E' τ := by
+intro τ
+have hstep : Unification_Step σ E E' := Unify_Step E E' σ σ' algo
+exact unifier_eq_step E E' σ hstep τ
+
+
+--------------------------------------------------------------------------
+--Theorem 3.10.4
+-- 2. If E (Naive_Standard_Unification) -> ⊥, then E is not unifiable
+--------------------------------------------------------------------------
+
+lemma uneq_none {sig : Signature} {X : Variables} [DecidableEq X] [BEq sig.funs] (E : EqualityProblem sig X)
+(σ : Substitution sig X) (hσ : Unifiable E) : Naive_Standard_Unification_Rec E initSubst ≠ none := by
+sorry
+
+lemma non_unifiable {sig : Signature} {X : Variables} [DecidableEq X] [BEq sig.funs] (E : EqualityProblem sig X)
+(h_none : Naive_Standard_Unification_Rec E initSubst = none) : ¬(Unifiable E) := by
+intro hUnif
+rcases hUnif with ⟨σ, hσ⟩
+have huneq_none : (Naive_Standard_Unification_Rec E initSubst ≠ none) := (uneq_none E σ (hσ := ⟨σ,hσ⟩))
+exact huneq_none h_none
+
+----------------------------------------------------------------------------------
+--Theorem 3.10.4
+-- 3. If E (Naive_Standard_Unification) -> E′(Solved_Form), then σE is a MGU of E
+----------------------------------------------------------------------------------
+
+lemma Solved_Form_Then_MGU {sig : Signature} {X : Variables} [DecidableEq X] (E E' : EqualityProblem sig X) (σE : Substitution sig X)
+(solved : (Solved_Form E')) (τ_eq : (∀ τ, Unifier E τ ↔ Unifier E' τ)) (hσ : (σE = Sigma_Solved E')):
+MostGeneralUnifier E σE := by
+
+subst hσ
+have mgs_solved : MostGeneralUnifier E' (Sigma_Solved E') := Most_General_Sigma_Solved E' solved
+rcases mgs_solved with ⟨hU', hmgu⟩
+
+constructor
+· exact (τ_eq (Sigma_Solved E')).mpr hU'
+· intro τ hτ
+  have Unifier_E' : Unifier E' τ := (τ_eq τ).mp hτ
+  exact hmgu τ Unifier_E'
+
+-----------------------------------------------------------------------------
+--Unifiable E ↔ ∃ σ : Substitution sig X, σ.domain ∪ σ.codomain ⊆ E.freeVars
+-----------------------------------------------------------------------------
+
+lemma E'_freeVars_Subset_E_freeVars {sig : Signature} {X : Variables} [DecidableEq X] [BEq sig.funs] (E E' : EqualityProblem sig X)
+(σ σ': Substitution sig X) (hUNIF : Unification_Step σ E E') : E'.freeVars ⊆ E.freeVars := by
+intro x hx
+induction hUNIF with
+| refl t E => simp_all
+| decomposition f args bargs E hlen => sorry
+| var_left x t E σ not_in => sorry
+| var_right x t E σ not_in => sorry
+
+lemma Solved_Dom_Subset_fV  {sig : Signature} {X : Variables} [DecidableEq X] [BEq sig.funs]
+(E : EqualityProblem sig X) (solved : Solved_Form E) : (Sigma_Solved E).domain ⊆ E.freeVars := by
+
+induction E with
+| nil => simp [Sigma_Solved]
+| cons eq E ih =>
+
+  rcases eq with ⟨s,t⟩
+  have varx : ∃ x, s = Term.var x := solved.left s t (by simp)
+  rcases varx with ⟨x,hx⟩
+
+  intro y hy
+  simp [Sigma_Solved, hx] at hy
+
+  by_cases eq_yx : y = x
+
+  · simp_all
+  · have y_in_dom : y ∈ (Sigma_Solved E).domain := by simp_all
+
+    have hsolved : Solved_Form E := by
+      rcases solved with ⟨h₁, h₂, h₃⟩
+      refine ⟨?_, ?_, ?_⟩
+      · intro s t eqE
+        exact h₁ s t (by simp [eqE])
+      · intro x' t₁ t₂ ht₁ ht₂
+        exact h₂ x' t₁ t₂ (by simp [ht₁]) (by simp [ht₂])
+      · intro x' t eqE
+        exact h₃ x' t (by simp [eqE])
+
+    have y_in_fV : y ∈ EqualityProblem.freeVars ((s,t) :: E) := by
+      have hy_in_fV : y ∈ EqualityProblem.freeVars E := ih hsolved y_in_dom
+      simp [hy_in_fV]
+
+    exact y_in_fV
+
+lemma Solved_Codom_Subset_fV {sig : Signature} {X : Variables} [DecidableEq X] [BEq sig.funs]
+(E : EqualityProblem sig X) (solved: Solved_Form E) : (Sigma_Solved E).codomain ⊆ E.freeVars := by
+
+induction E with
+| nil => simp [Sigma_Solved]
+| cons eq E ih =>
+
+  rcases eq with ⟨s,t⟩
+  have varx : ∃ x, s = Term.var x := solved.left s t (by simp)
+  rcases varx with ⟨x,hx⟩
+
+  intro y hy
+  simp [Sigma_Solved, hx] at hy
+
+  by_cases eq_yx : y = x
+
+  · simp_all
+  · have y_in_dom : y ∈ (Sigma_Solved E).codomain := sorry
+
+    have hsolved : Solved_Form E := by
+      rcases solved with ⟨h₁, h₂, h₃⟩
+      refine ⟨?_, ?_, ?_⟩
+      · intro s t eqE
+        exact h₁ s t (by simp [eqE])
+      · intro x' t₁ t₂ ht₁ ht₂
+        exact h₂ x' t₁ t₂ (by simp [ht₁]) (by simp [ht₂])
+      · intro x' t eqE
+        exact h₃ x' t (by simp [eqE])
+
+    have y_in_fV : y ∈ EqualityProblem.freeVars ((s,t) :: E) := by
+      have hy_in_fV : y ∈ EqualityProblem.freeVars E := ih hsolved y_in_dom
+      simp [hy_in_fV]
+
+    exact y_in_fV
+
+lemma do_codom_subset_E {sig : Signature} {X : Variables} [DecidableEq X] [BEq sig.funs] (E : EqualityProblem sig X) (σ σ' : Substitution sig X)
+(algo : Naive_Standard_Unification_Rec E initSubst = some σ') : σ'.domain ∪ σ'.codomain ⊆ E.freeVars := by sorry
+
+
+---------------------------------------------------------
+--Unifiable E ↔ ∃ σ : Substitution sig X, Idempotent σ
+---------------------------------------------------------
+
+lemma σ_solved_dom_codom_disj {sig : Signature} {X : Variables} [DecidableEq X] [BEq sig.funs] (E : EqualityProblem sig X) (solved : Solved_Form E) :
+(Sigma_Solved E).domain ∩ (Sigma_Solved E).codomain = ∅ := by
+sorry
+
+lemma new_idempotent {sig : Signature} {X : Variables} [DecidableEq X] [BEq sig.funs]
+(E : EqualityProblem sig X) (solved : Solved_Form E) : Idempotent (Sigma_Solved E) := by
+apply (idempotent_iff_inter_empty (σ := Sigma_Solved E)).mpr
+exact σ_solved_dom_codom_disj E solved
+
+------------------------------------------
+-- Main Unfication Theorem --
+------------------------------------------
+
+theorem unifiable_iff_mgu_idempot {sig : Signature} {X : Variables} [DecidableEq X] [BEq sig.funs] [BEq (Equality sig X)] [LawfulBEq (Equality sig X)]
+(E : EqualityProblem sig X) : Unifiable E ↔ ∃ σ : Substitution sig X, MostGeneralUnifier E σ ∧ Idempotent σ ∧ σ.domain ∪ σ.codomain ⊆ E.freeVars := by
+
+  constructor
+
+  · intro hunif
+    rcases hunif with ⟨σ, hσ⟩
+    cases halgo' : Naive_Standard_Unification_Rec E initSubst with
+
+    | none =>
+       have nnot := uneq_none E σ (hσ := ⟨σ,hσ⟩)
+       exact (nnot halgo').elim
+
+    | some σ_out =>
+      obtain ⟨hE', hE'_solved, σ_solved⟩ := Ex_SolvedForm_Sigma E σ_out halgo'
+      subst σ_solved
+
+      have mgu_he' : MostGeneralUnifier hE' (Sigma_Solved hE') := Most_General_Sigma_Solved hE' hE'_solved
+      have heq_τ : ∀ τ, Unifier E τ ↔ Unifier hE' τ := sorry
+      have hmgu : MostGeneralUnifier E (Sigma_Solved hE') := sorry
+
+      have hidempotent : Idempotent (Sigma_Solved hE') := new_idempotent hE' hE'_solved
+
+      have dom_codom_fV : ((Sigma_Solved hE').domain ∪ (Sigma_Solved hE').codomain) ⊆ E.freeVars := sorry
+
+      exact ⟨Sigma_Solved hE', hmgu, hidempotent, dom_codom_fV⟩
+
+  · intro h
+    obtain ⟨σ, ⟨⟨⟩⟩⟩ := h
+    use σ
+
+alias main_unification_theorem := unifiable_iff_mgu_idempot
